WIP more precise raw items

src/cbor/CBOR.Spec.Raw.fsti
@@ -6,17 +6,107 @@ module U64 = FStar.UInt64
 
 (* Raw data items, disregarding ordering of map entries *)
 
+let nlist ([@@@strictly_positive] t: eqtype) (n: nat) : Tot eqtype = (l: list t { List.Tot.length l == n })
+
+type integer_size = (n: nat { n < 4 })
+
+open FStar.Mul
+
+type raw_uint64 = {
+  size: integer_size;
+  value: (x: U64.t { U64.v x < pow2 (8 * pow2 size) })
+}
+
+let _ = assert_norm (8 * pow2 3 == 64)
+
 type raw_data_item : eqtype
 = | Simple: (v: simple_value) -> raw_data_item
-  | Int64: (typ: major_type_uint64_or_neg_int64) -> (v: U64.t) -> raw_data_item
-  | String: (typ: major_type_byte_string_or_text_string) -> (v: Seq.seq U8.t { FStar.UInt.fits (Seq.length v) U64.n }) -> raw_data_item // Section 3.1: "a string containing an invalid UTF-8 sequence is well-formed but invalid", so we don't care about UTF-8 specifics here.
-  | Array: (v: list raw_data_item { FStar.UInt.fits (List.Tot.length v) U64.n }) -> raw_data_item
-  | Map: (v: list (raw_data_item & raw_data_item) { FStar.UInt.fits (List.Tot.length v) U64.n }) -> raw_data_item
-  | Tagged: (tag: U64.t) -> (v: raw_data_item) -> raw_data_item
+  | Int64: (typ: major_type_uint64_or_neg_int64) -> (v: raw_uint64) -> raw_data_item
+  | String: (typ: major_type_byte_string_or_text_string) -> (len: raw_uint64) -> (v: Seq.lseq U8.t (U64.v len.value)) -> raw_data_item // Section 3.1: "a string containing an invalid UTF-8 sequence is well-formed but invalid", so we don't care about UTF-8 specifics here.
+  | Array: (len: raw_uint64) -> (v: nlist raw_data_item (U64.v len.value)) -> raw_data_item
+  | Map: (len: raw_uint64) -> (v: nlist (raw_data_item & raw_data_item) (U64.v len.value)) -> raw_data_item
+  | Tagged: (tag: raw_uint64) -> (v: raw_data_item) -> raw_data_item
 //  | Float: (v: Float.float) -> raw_data_item // TODO
 
 let dummy_raw_data_item : Ghost.erased raw_data_item =
-  Int64 cbor_major_type_uint64 0uL
+  Int64 cbor_major_type_uint64 { size = 0; value = 0uL }
+
+let raw_uint64_equiv (x1 x2: raw_uint64) : Tot bool =
+  x1.value = x2.value
+
+let rec list_forall2 (#t1 #t2: Type) (l1: list t1) (l2: list t2) (p: (x1: t1) -> (x2: t2 { x1 << l1 /\ x2 << l2 }) -> bool) : Tot bool (decreases l1) =
+  match l1, l2 with
+  | [], [] -> true
+  | a1 :: q1, a2 :: q2 -> p a1 a2 && list_forall2 q1 q2 p
+  | _ -> false
+
+(*
+let rec list_forall (#t: Type) (l: list t) (p: (x: t { x << l }) -> bool) : bool =
+  match l with
+  | [] -> true
+  | a :: q -> p a && list_forall q p
+
+let rec list_exists (#t: Type) (l: list t) (p: (x: t { x << l }) -> bool) : bool =
+  match l with
+  | [] -> false
+  | a :: q -> p a || list_exists q p
+
+let list_exists2 (#t': Type) (l0: list t') (#t: Type) (l: list t) (p: (x': t') -> (x: t { x' << l0 /\ x << l }) -> bool) (x: t' { x << l0 }) : bool =
+  list_exists l (p x)
+
+let list_exists1_swap (#t': Type) (#t: Type) (l: list t) (p: (x: t) -> (x': t' { x << l }) -> bool) (x: t') : bool =
+  list_exists l (fun x' -> p x' x)
+
+let rec raw_equiv (l1 l2: raw_data_item) : Tot bool (decreases l1) =
+  match l1, l2 with
+  | Simple v1, Simple v2 -> v1 = v2
+  | Int64 ty1 v1, Int64 ty2 v2 -> ty1 = ty2 && raw_uint64_equiv v1 v2
+  | String ty1 len1 v1, String ty2 len2 v2 -> ty1 = ty2 && raw_uint64_equiv len1 len2 && v1 = v2
+  | Array len1 v1, Array len2 v2 -> raw_uint64_equiv len1 len2 && list_forall2 v1 v2 raw_equiv
+  | Map len1 v1, Map len2 v2 ->
+    raw_uint64_equiv len1 len2 &&
+    list_forall v1 (list_exists2 v1 v2 raw_pair_equiv) &&
+    list_forall v2 (list_exists1_swap v1 raw_pair_equiv)
+  | Tagged tag1 v1, Tagged tag2 v2 ->
+    raw_uint64_equiv tag1 tag2 &&
+    raw_equiv v1 v2
+  | _ -> false
+
+and raw_pair_equiv (l1 l2: (raw_data_item & raw_data_item)) : Tot bool (decreases l1) =
+  raw_equiv (fst l1) (fst l2) && raw_equiv (snd l1) (snd l2)
+*)
+
+val raw_equiv (l1 l2: raw_data_item) : Tot bool
+
+noextract
+let holds_on_pair2
+  (#t: Type)
+  (pred: (t -> t -> bool))
+  (x: (t & t))
+  (y: (t & t))
+: Tot bool
+= let (x1, x2) = x in
+  let (y1, y2) = y in
+  pred x1 y1 && pred x2 y2
+
+let list_for_all_exists (#t1 #t2: Type) (p: t1 -> t2 -> bool) (l1: list t1) (l2: list t2) : bool =
+  List.Tot.for_all (fun x -> List.Tot.existsb (p x) l2) l1
+
+val raw_equiv_eq (l1 l2: raw_data_item) : Lemma
+  (raw_equiv l1 l2 == begin match l1, l2 with
+  | Simple v1, Simple v2 -> v1 = v2
+  | Int64 ty1 v1, Int64 ty2 v2 -> ty1 = ty2 && raw_uint64_equiv v1 v2
+  | String ty1 len1 v1, String ty2 len2 v2 -> ty1 = ty2 && raw_uint64_equiv len1 len2 && v1 = v2
+  | Array len1 v1, Array len2 v2 -> raw_uint64_equiv len1 len2 && list_forall2 v1 v2 raw_equiv
+  | Map len1 v1, Map len2 v2 ->
+    raw_uint64_equiv len1 len2 &&
+    list_for_all_exists (holds_on_pair2 raw_equiv) v1 v2 &&
+    list_for_all_exists (holds_on_pair2 raw_equiv) v2 v1
+  | Tagged tag1 v1, Tagged tag2 v2 ->
+    raw_uint64_equiv tag1 tag2 &&
+    raw_equiv v1 v2
+  | _ -> false
+  end)
 
 noextract
 let get_major_type
@@ -25,16 +115,10 @@ let get_major_type
 = match d with
   | Simple _ -> cbor_major_type_simple_value
   | Int64 m _ -> m
-  | String m _ -> m
-  | Array _ -> cbor_major_type_array
-  | Map _ -> cbor_major_type_map
+  | String m _ _ -> m
+  | Array _ _ -> cbor_major_type_array
+  | Map _ _ -> cbor_major_type_map
   | Tagged _ _ -> cbor_major_type_tagged
-
-noextract
-val holds_on_raw_data_item
-  (p: (raw_data_item -> bool))
-  (x: raw_data_item)
-: Tot bool
 
 noextract
 let holds_on_pair
@@ -46,14 +130,20 @@ let holds_on_pair
   pred x1 && pred x2
 
 noextract
+val holds_on_raw_data_item
+  (p: (raw_data_item -> bool))
+  (x: raw_data_item)
+: Tot bool
+
+noextract
 let holds_on_raw_data_item'
   (p: (raw_data_item -> bool))
   (x: raw_data_item)
 : Tot bool
 = p x &&
   begin match x with
-  | Array l -> List.Tot.for_all (holds_on_raw_data_item p) l
-  | Map l ->
+  | Array _ l -> List.Tot.for_all (holds_on_raw_data_item p) l
+  | Map _ l ->
     List.Tot.for_all (holds_on_pair (holds_on_raw_data_item p)) l
   | Tagged _ v -> holds_on_raw_data_item p v
   | _ -> true
@@ -76,7 +166,7 @@ let holds_on_raw_data_item_eq_simple
 let holds_on_raw_data_item_eq_int64
   (p: (raw_data_item -> bool))
   (typ: major_type_uint64_or_neg_int64)
-  (v: U64.t)
+  (v: raw_uint64)
 : Lemma
   (holds_on_raw_data_item p (Int64 typ v) == p (Int64 typ v))
   [SMTPat (holds_on_raw_data_item p (Int64 typ v))]
@@ -85,31 +175,34 @@ let holds_on_raw_data_item_eq_int64
 let holds_on_raw_data_item_eq_string
   (p: (raw_data_item -> bool))
   (typ: major_type_byte_string_or_text_string)
-  (v: Seq.seq U8.t { FStar.UInt.fits (Seq.length v) U64.n })
+  (len: raw_uint64)
+  (v: Seq.lseq U8.t (U64.v len.value))
 : Lemma
-  (holds_on_raw_data_item p (String typ v) == p (String typ v))
-  [SMTPat (holds_on_raw_data_item p (String typ v))]
-= holds_on_raw_data_item_eq p (String typ v)
+  (holds_on_raw_data_item p (String typ len v) == p (String typ len v))
+  [SMTPat (holds_on_raw_data_item p (String typ len v))]
+= holds_on_raw_data_item_eq p (String typ len v)
 
 let holds_on_raw_data_item_eq_array
   (p: (raw_data_item -> bool))
-  (v: list raw_data_item { FStar.UInt.fits (List.Tot.length v) U64.n })
+  (len: raw_uint64)
+  (v: nlist raw_data_item (U64.v len.value))
 : Lemma
-  (holds_on_raw_data_item p (Array v) == (p (Array v) && List.Tot.for_all (holds_on_raw_data_item p) v))
-  [SMTPat (holds_on_raw_data_item p (Array v))]
-= holds_on_raw_data_item_eq p (Array v)
+  (holds_on_raw_data_item p (Array len v) == (p (Array len v) && List.Tot.for_all (holds_on_raw_data_item p) v))
+  [SMTPat (holds_on_raw_data_item p (Array len v))]
+= holds_on_raw_data_item_eq p (Array len v)
 
 let holds_on_raw_data_item_eq_map
   (p: (raw_data_item -> bool))
-  (v: list (raw_data_item & raw_data_item) { FStar.UInt.fits (List.Tot.length v) U64.n })
+  (len: raw_uint64)
+  (v: nlist (raw_data_item & raw_data_item) (U64.v len.value))
 : Lemma
-  (holds_on_raw_data_item p (Map v) == (p (Map v) && List.Tot.for_all (holds_on_pair (holds_on_raw_data_item p)) v))
-  [SMTPat (holds_on_raw_data_item p (Map v))]
-= holds_on_raw_data_item_eq p (Map v)
+  (holds_on_raw_data_item p (Map len v) == (p (Map len v) && List.Tot.for_all (holds_on_pair (holds_on_raw_data_item p)) v))
+  [SMTPat (holds_on_raw_data_item p (Map len v))]
+= holds_on_raw_data_item_eq p (Map len v)
 
 let holds_on_raw_data_item_eq_tagged
   (p: (raw_data_item -> bool))
-  (tag: U64.t)
+  (tag: raw_uint64)
   (v: raw_data_item)
 : Lemma
   (holds_on_raw_data_item p (Tagged tag v) <==> (p (Tagged tag v) && holds_on_raw_data_item p v))
@@ -127,15 +220,119 @@ let map_entry_order
 = key_order (fst m1) (fst m2)
 
 noextract
-let data_item_wf_head (order: (raw_data_item -> raw_data_item -> bool)) (x: raw_data_item) : Tot bool
+let raw_data_item_sorted_elem (order: (raw_data_item -> raw_data_item -> bool)) (x: raw_data_item) : Tot bool
 = match x with
-  | Map l ->
+  | Map _ l ->
       FStar.List.Tot.sorted (map_entry_order order _) l
   | _ -> true
 
 noextract
-let data_item_wf (order: (raw_data_item -> raw_data_item -> bool)) : Tot (raw_data_item -> bool)
-= holds_on_raw_data_item (data_item_wf_head order)
+let raw_data_item_sorted (order: (raw_data_item -> raw_data_item -> bool)) : Tot (raw_data_item -> bool)
+= holds_on_raw_data_item (raw_data_item_sorted_elem order)
 
-let data_item (order: (raw_data_item -> raw_data_item -> bool)) =
-  (x: raw_data_item { data_item_wf order x == true })
+let raw_uint64_optimal (x: raw_uint64) : Tot bool =
+  if x.size = 0
+  then true
+  else pow2 (8 * pow2 (x.size - 1)) <= U64.v x.value
+
+let raw_uint64_optimal_unique (x1 x2: raw_uint64) : Lemma
+  (requires (raw_uint64_optimal x1 /\ raw_uint64_optimal x2 /\ raw_uint64_equiv x1 x2))
+  (ensures (x1 == x2))
+= ()
+
+let rec raw_uint64_optimize (x: raw_uint64) : Pure raw_uint64
+  (requires True)
+  (ensures (fun x' -> raw_uint64_equiv x x' /\ raw_uint64_optimal x'))
+  (decreases x.size)
+= if x.size = 0
+  then x
+  else if pow2 (8 * pow2 (x.size - 1)) <= U64.v x.value
+  then x
+  else raw_uint64_optimize { x with size = x.size - 1 }
+
+let raw_data_item_ints_optimal_elem (x: raw_data_item) : Tot bool =
+  match x with
+  | Int64 _ v
+  | String _ v _
+  | Array v _
+  | Map v _
+  | Tagged v _
+    -> raw_uint64_optimal v
+  | Simple _ -> true
+
+let raw_data_item_ints_optimal (x: raw_data_item) : Tot bool =
+  holds_on_raw_data_item raw_data_item_ints_optimal_elem x
+
+let rec list_no_setoid_repeats
+  (#t: Type)
+  (equiv: t -> t -> bool)
+  (l: list t)
+: Tot bool
+  (decreases l)
+= match l with
+  | [] -> true
+  | [_] -> true
+  | a :: q ->
+    list_no_setoid_repeats equiv q &&
+    not (List.Tot.existsb (equiv a) q)
+
+let valid_raw_data_item_elem
+  (l: raw_data_item)
+: Tot bool
+= match l with
+  | Map _ v -> list_no_setoid_repeats (holds_on_pair2 raw_equiv) v
+  | _ -> true
+
+let valid_raw_data_item
+  (l: raw_data_item)
+: Tot bool
+= holds_on_raw_data_item valid_raw_data_item_elem l
+
+let order_irrefl
+  (#t: Type)
+  (order: t -> t -> bool)
+: Tot prop
+= forall x . ~ (order x x)
+
+let order_trans
+  (#t: Type)
+  (order: t -> t -> bool)
+: Tot prop
+= forall x y z . (order x y /\ order y z) ==> order x z
+
+let rec raw_equiv_sorted_optimal
+  (order: raw_data_item -> raw_data_item -> bool {
+    order_irrefl order /\
+    order_trans order
+  })
+  (x1 x2: raw_data_item)
+: Lemma
+  (requires (
+    raw_equiv x1 x2 /\
+    raw_data_item_sorted order x1 /\
+    raw_data_item_sorted order x2 /\
+    raw_data_item_ints_optimal x1 /\
+    raw_data_item_ints_optimal x2
+  ))
+  (ensures (x1 == x2))
+  (decreases x1)
+= raw_equiv_eq x1 x2;
+  match x1, x2 with
+  | Simple _, Simple _ -> ()
+  | Int64 _ v1, Int64 _ v2 ->
+    raw_uint64_optimal_unique v1 v2
+  | _ -> admit ()
+
+let raw_data_item_sorted_optimal_valid
+  (order: raw_data_item -> raw_data_item -> bool {
+    order_irrefl order /\
+    order_trans order
+  })
+  (x1: raw_data_item)
+: Lemma
+  (requires (
+    raw_data_item_sorted order x1 /\
+    raw_data_item_ints_optimal x1
+  ))
+  (ensures (valid_raw_data_item x1))
+= admit ()
